\appendix
\chapter{Haskell Implementation--main algorithm}\label{ap:a}
\begin{verbatim}


--predicate to string
pretostring :: Predicate -> String
pretostring (TP x y) = "(" ++ pretostring x ++ "->" ++ pretostring y ++ ")"
pretostring (TVar (x:xs)) | xs == [] = [x]
                          | otherwise = [x] ++ "->" ++ (pretostring (TVar xs))
                          
--statement to string
stat_to_string :: Statement -> String
stat_to_string (x, y) = (tostring x) ++ ":" ++ (pretostring y)

--context to string
context_to_string :: Context -> String
context_to_string (x:xs) | xs == [] = stat_to_string x
| otherwise = stat_to_string x ++ ", " ++ context_to_string xs
context_to_string [] = []

{-|
Type assignment mechanism
-}
--derivation rules, not used for principal pair algorithm.
drules :: [Derivation] -> Statement
--rules I
drules ((context, (Var x, TVar (pre1:[])):[], (m, TVar (pre2:[]))):[]) 
           = ((Abs x m), TP (TVar [pre1]) (TVar [pre2]))
--rule E
drules ((context1, [], (m1, TVar [a, b]) ):[(context2, [], (m2, TVar [a2]))]) 
      | (context1 == context2 && a == a2) = ((App m1 m2), TVar [b])


--evaluate a term and the type
eval_type :: Term -> Context -> Statement
eval_type (App (App x y) t) context =
           drules ((context, [], (s1, p1)):[(context, [], (s2, p2))])
                    where (s1, p1) = eval_type (App x y) context
                          (s2, p2) = eval_type t context
eval_type (App (Abs x y) t) context = 
           drules ((context, [], (s1, p1)):[(context, [], (s2, p2))])
                    where (s1, p1) = eval_type (Abs x y) context
                          (s2, p2) = eval_type t context
eval_type (App (Var x) t) context = 
           drules ((context, [], (s1, p1)):[(context, [], (s2, p2))])
                    where (s1, p1) = search (Var x) context
                          (s2, p2) = eval_type t context
eval_type (Var x) context = search (Var x) context
eval_type (Abs x t) context = 
          drules ((context, (s1, p1):[], (s2, p2)):[])
                   where (s1, p1) = search (Var x) context
                         (s2, p2) = eval_type t context
                         
--type substitution
type_subs :: TSub -> Type -> Type
type_subs (Sub((TVar [f]), c)) (TVar [x]) | [x] == [f] = c
                                          | otherwise = TVar [x]
type_subs (Sub((TVar [f]), c)) (TP a b) = TP (type_subs (Sub((TVar [f]), c)) a)
                               (type_subs (Sub((TVar [f]), c)) b)
type_subs (So (s1, s2)) x = so (So (s1, s2)) x

--So
so :: TSub -> Type -> Type
so (So(s1, s2)) a = type_subs s1 (type_subs s2 a)

--context substitution
context_sub :: TSub -> Context -> Context
context_sub (Sub (s, t)) ((x, y):[]) = [(x, (type_subs (Sub(s, t)) y))]
context_sub (Sub (s, t)) ((x, y):cx) = (x, (type_subs (Sub(s, t)) y)):
                                         (context_sub (Sub (s, t)) cx)
context_sub (So (s1, s2)) ((x, y):[]) = [(x, (type_subs (So(s1, s2)) y))]
context_sub (So (s1, s2)) ((x, y):cx) = (x, (so (So(s1, s2)) y)):
                                      (context_sub (So (s1, s2)) cx)
context_sub _ [] = []

--Robinson's Unification Algorithm
unify :: Type -> Type -> TSub
unify (TVar [x]) (TVar [y]) = Sub (TVar [x], TVar [y])
unify (TVar [x]) (TP a b) | not (occur (TVar [x]) a) && not (occur (TVar [x]) b) 
                            = Sub (TVar [x], TP a b)
                          | otherwise = Sub (TVar "A", TVar "A")
unify (TP a b) (TVar [x]) = unify (TVar [x]) (TP a b)
unify (TP a b) (TP c d) = So (s2, s1)
                          where s1 = unify a c
                                s2 = unify (type_subs s1 b) (type_subs s1 d)

--context unification
unify_contexts :: Context-> Context -> TSub
unify_contexts ((x, a):g0) g1 | pre /= (TVar []) = So (s2, s1)
                              | otherwise = unify_contexts g0 g1
                              where (_, pre) = search x g1
                                          s1 = unify a pre
                                          s2 = unify_contexts (context_sub s1 g0) 
                                                   (context_sub s1 g1)
unify_contexts [] _ = Sub (TVar "A", TVar "A")

--search a term in a context, return the statement
search :: Term -> Context -> Statement
search t ((s, p):cx) | t == s = (s, p)
                     | otherwise = search t cx
search _ [] = (Var ' ', TVar [])

--checks whether a context contains a statement for a term
contains :: Term -> Context -> Bool
contains t ((s, _):[]) | t == s = True
                       | otherwise = False
contains t ((s, _):cx) | t == s = True
                       | otherwise = contains t cx
contains _ [] = False


--PRINCIPAL PAIR ALGORITHM
ppc :: Term -> [Char] -> (PPc, [Char])
ppc (Var x) r = (([(Var x, f)], f), tl)
                 where (f, tl) = fresh r
ppc (Abs x y) r | contains (Var x) pi = ((removeItem (Var x, a) pi, (TP a p)), tl1)
                | otherwise = ((pi, (TP f p)), tl1)
                where (f, tl) = fresh r
                      ((pi, p), tl1) = ppc y tl
                      (_, a) = search (Var x) pi
ppc (App m n) r = ((context_sub s2 (context_sub s1 (pi1++pi2)), 
                      type_subs s2 (type_subs s1 f)), tl2)
                  where (f, tl) = fresh r
                        ((pi1, p1), tl1)= ppc m tl
                        ((pi2, p2), tl2)= ppc n tl1
                         s1 = unify p1 (TP p2 f)
                         s2 = unify_contexts (context_sub s1 pi1) 
                                   (context_sub s1 pi2)

--get a fresh type from the recorder
fresh :: [Char] -> (Type, [Char])
fresh x = (TVar [(head x)], tail x)

--check whether a single type variable occurs in another type
occur :: Type -> Type -> Bool
occur (TVar [x]) (TP a b) = occur (TVar [x]) a || occur (TVar [x]) b
occur (TVar [x]) (TVar (a:ax)) | x == a = True
                               | otherwise = occur (TVar [x]) (TVar ax)
occur _ (TVar []) = False

--recursive evaluation
recur_eval :: Term -> IO()
recur_eval t | evalnormal t == t = putStrLn("")
             | otherwise = do
                           putStrLn("==> "++ tostring term)
                           recur_eval term
                             where term = evalnormal t

--recursive evaluation xgc
recur_evalxgc :: Term -> IO()
recur_evalxgc t | evalxgc t == t = putStrLn("")
                | otherwise = do
                              putStrLn("==> "++ tostring term)
                              recur_evalxgc term
                                where term = evalxgc t


--lambda calculus

--remove an element from a list
removeItem :: Eq a => a -> [a] -> [a]
removeItem _ [] = []
removeItem x (y:xs) = if x == y then removeItem x xs
                      else y:(removeItem x xs)

--the set of free variables of a lambda term
freevar :: Term -> [Term]
freevar (Var x) = (Var x):[]
freevar (App x y) = (freevar x) ++ (freevar y)
freevar (Abs y m) = if (Var y) `elem` (freevar m) then 
                              removeItem (Var y) (freevar m)
else (freevar m)
freevar (XSub m from to) = (removeItem from (freevar m)) ++ (freevar to)

--normal order
evalnormal :: Term -> Term
evalnormal (Var x) = Var x
evalnormal (Abs x t) = (Abs x (evalnormal t))
evalnormal (App (Abs x t) v) = subs t (Var x, v)
evalnormal (App x t) | x == evalnormal x = (App x (evalnormal t))
                     | otherwise = (App (evalnormal x) t)

--call-by-name reduction
evalcbn :: Term -> Term
evalcbn (Var x) = Var x
evalcbn (Abs x t) = (Abs x t)
evalcbn (App (Abs x t) v) = subs t (Var x, v)
evalcbn (App x y) | x == evalcbn x = (App x y)
                  | otherwise = (App (evalcbn x) y)

--call-by-value reduction
evalcbv :: Term -> Term
evalcbv (Var x) = Var x
evalcbv (Abs x t) = (Abs x t)
evalcbv (App (Abs x t) y) | y == evalcbv y = subs t (Var x, y)
                          | otherwise = App (Abs x t) (evalcbv y)
evalcbv (App x y) | x == evalcbv x = (App x (evalcbv y))
                  | otherwise = (App (evalcbv x) y)

--head reduction
headreduction :: Term -> Term
headreduction (Var x) = Var x
headreduction (Abs x t) = (Abs x (headreduction t))
headreduction (App (Abs x t) y) = subs t (Var x, y)
headreduction (App x y) | x == headreduction x = (App x y)
                        | otherwise = (App (headreduction x) y)

--call-by-value reduction
apporder :: Term -> Term
apporder (Var x) = Var x
apporder (Abs x t) = (Abs x (apporder t))
apporder (App (Abs x t) y) | apporder (Abs x t) /= (Abs x t) 
                             = (App (apporder (Abs x t)) y)
                           | apporder (Abs x t) == (Abs x t) && 
                              apporder y /= y 
                             = (App (Abs x t) (apporder y))
                           | apporder (Abs x t) == (Abs x t) && 
                              apporder y == y 
                              = subs t (Var x, y)
apporder (App x y) | x == apporder x = (App x (apporder y))
                   | otherwise = (App (apporder x) y)

--evaluate a xgc-term
evalxgc :: Term -> Term
evalxgc (App (Abs x t) v) = XSub t (Var x) v
evalxgc (App x t) | x == evalxgc x = (App x (evalxgc t))
                  | otherwise = (App (evalxgc x) t)
evalxgc (Var x) = Var x
evalxgc (Abs x t) = (Abs x (evalxgc t))
evalxgc (XSub (Var x) from to) = if (Var x) == from then to
                                 else (Var x)
evalxgc (XSub (Abs x m) from to) = if from `elem` (freevar (Abs x m)) then 
                                      Abs x (XSub m from to)
                                   else (Abs x m)
evalxgc (XSub (App x y) from to) = if from `elem` (freevar (App x y)) then 
                                      App (XSub x from to) (XSub y from to)
                                   else (App x y)
evalxgc (XSub (XSub x f t) from to) = if from `elem` (freevar (XSub x f t)) then 
                                       XSub (evalxgc (XSub x f t)) from to
                                      else (XSub x f t)


--Term susbstitution
subs :: Term -> (Term, Term) -> Term
subs (Var x) (Var y, t) | x == y = t
                        | x /=y = Var x
subs (Abs y m) (Var x, n) | not ((Var y) `elem` (freevar n)) && y /= x 
                            = Abs y (subs m (Var x, n))
                          | y == x = Abs y m
                          | (Var y) `elem` (freevar n) && y/= x 
                            = Abs 'z' (subs (subs m (Var y, Var 'z')) (Var x, n) )
subs (App p q) (Var y, n) = App (subs p (Var y, n)) (subs q (Var y, n))

--print a term
tostring :: Term -> String
tostring (Var x) = [x]
tostring (Abs x y) = "(/" ++ [x] ++ "." ++ (tostring y) ++ ")"
tostring (App x y) = "(" ++ tostring x ++ tostring y ++ ")"
tostring (XSub m from to) = tostring m ++ "<" ++ tostring from ++ 
                             " := " ++ tostring to ++ ">"

\end{verbatim}